theories/pop_cost.v
@@ -20,10 +20,12 @@ Section proof.
       pop_nonempty (#ℓ)
     {{{ d', RET (x, d')%V; isDeque π depth oD d' ∗ Token π depth }}}.
   Proof.
+    Opaque isPopFiveTuple isUnsafePopFiveTuple prepare_pop naive_pop.
     iIntros (depth ψ) "(Hd & τ & O) Hψ".
     rewrite isDeque_unfold.
     rewrite /pop_nonempty.
-    iLöb as "iH" forall (ℓ oD x depth).
+    Opaque pop_nonempty.
+    iLöb as "iH" forall (ℓ oD x depth ψ).
     iDestruct "Hd" as "[[%H _] | (%ℓ' & %Heqℓ & Hℓ)]". by inversion H.
     inversion Heqℓ as [H]. rewrite -H. clear Heqℓ H ℓ'.
     wp_pures.
@@ -36,695 +38,120 @@ Section proof.
     wp_pures.
     2: {
       wp_pures.
-      (* NOTE(Juliette): pourquoi nommer la première hypothèse casse tout ????? je ne comprends rien *)
-      iDestruct "Safe" as "[Hsafe pop_safe]".
-      wp_bind (naive_pop_safe d)%E.
-      iApply (wp_wand with "pop_safe").
-      iIntros (true_) "->".
-      wp_apply (naive_pop_safe with "Hd").
-
-    }
-    (*
-    iDestruct (persist_structure with "πd") as "[#Hv
-        (%pr & %ld & %md & %rd & %sf & %prC & %ldC & %mdC & %rdC & %sfC
-            & %kPr & %kMd & %kSf & %ltr & %rtr & -> & %cfg & pot
-            & #Hpr & #Hld & #Hmd & #Hrd & #Hsf & #Hltr & #Hrtr & %Heq)]".
-    wp_pures.
-    *)
-    (* START HERE *)
-
-    (*
-    wp_bind (if: _ then _ else _)%E.
-    wp_apply (wp_strong_mono _ _ _ _ _
-      (λ v, isPopFiveTuple π depth (⋅x ++ oD) v ∗ Token π (S depth))%I
-      with "[O τ]"); [easy | easy | |]. {
-    wp_apply (bsize_better_spec with "Hmd") as "_".
-    wp_pures.
-    destruct (bool_decide (kMd = 0)) eqn:?.
-    { (* apply bool_decide_eq_true_1 in Heqb as Heqmd.
-      apply bool_decide_code_true in Heqb as ->.
-      wp_pures.
-      iDestruct (split_time 3 with "τ") as "[ι τ]". by lia.
-      iFrame.
-      inversion cfg; [| exfalso; lia].
-      destruct ldC; inversion H.
-      destruct rdC; inversion H1.
-      iDestruct (big_sepL2_nil_inv_l with "Hltr") as "->".
-      iDestruct (big_sepL2_nil_inv_l with "Hrtr") as "->".
-      iExists pr,ld,md,rd,sf,prC,[],mdC,[],sfC,0,0,kSf,[],[].
-      iFrame "#".
-      iSplitR. done.
-      iSplitR.
-        { iPureIntro.
-          rewrite Heqmd in cfg |- *.
-          invert_all_in; constructor; list_elem_of.
-        }
-      iSplitL. by iApply three_time_enough.
-      do 2 doneL.
-      done.
-      *)
-      admit.
-    }
-    apply bool_decide_eq_false_1 in Heqb as Heqmd.
-    apply bool_decide_code_false in Heqb as ->.
-    wp_pures.
-    wp_apply (bsize_better_spec with "Hpr") as "_".
-    wp_pures.
-    destruct (bool_decide (kPr = 3)) eqn:?.
-    2: { (*
-      apply bool_decide_eq_false_1 in Heqb as Heqpr.
-      apply bool_decide_code_false in Heqb as ->.
-      wp_pures.
-      iDestruct (split_time 3 with "τ") as "[ι τ]". by lia.
-      iFrame.
-      iExists pr,ld,md,rd,sf,prC,ldC,mdC,rdC,sfC,kPr,kMd,kSf,ltr,rtr.
-      iFrame "#".
-      iSplitR. done.
-      iSplitR.
-        { iPureIntro.
-          inversion cfg; [exfalso; lia |].
-          invert_all_in; constructor; list_elem_of.
-        }
-      iSplitL. by iApply three_time_enough.
-      iSplitR. iApply (big_sepL2_mono with "Hltr"). by auto.
-      iSplitR. iApply (big_sepL2_mono with "Hrtr"). by auto.
-      done.
-      *)
-      admit.
-    }
-    apply bool_decide_eq_true_1 in Heqb as Heqpr.
-    apply bool_decide_code_true in Heqb as ->.
-    wp_pures.
-    rewrite {1}isDeque_unfold {1}isDeque_unfold.
-    iDestruct "Hld" as "[[-> ->] | (%ℓld & -> & Hld)]";
-    iDestruct "Hrd" as "[[-> ->] | (%ℓrd & -> & Hrd)]";
-    wp_pures.
-    - (* wp_apply (bsize_better_spec with "Hsf") as "_".
-      wp_pures.
-      destruct (bool_decide (kSf = 3)) eqn:?.
-      + apply bool_decide_eq_true_1 in Heqb as Heqsf.
-        apply bool_decide_code_true in Heqb as ->.
-        wp_pures.
-        wp_bind (inject_whole_buffer _ _ _).
-        wp_apply (binject_whole_spec with "[Hmd Hsf]") as "%sf' #Hsf'".
-          by iFrame "#".
-        wp_apply (binject_whole_spec with "[Hmd Hsf']") as "%sf'' #Hsf''".
-          by iFrame "#".
+      iDestruct "Safe" as (kp ks) "(Hsafe & τ' & pop_safe)".
+      iDestruct "Hsafe" as "#Hsafe".
+      Ltac gather_t pot := iDestruct (time_combine with String.concat "" ["[τ "; pot; "]"]) as "τ"; [ iFrame |].
+      gather_t "τ'".
+      iAssert (isPersFiveTuple π depth (⋅x ++ oD) d) as "Hd".
+      - Transparent isPopFiveTuple.
+        iDestruct "Hsafe" as "(%p & %l & %m & %r & %s & %op & %ol & %om & %or & %os &
+                            %kMd & %ltr & %rtr &
+                            -> & %conf & #Hp & #Hl & #Hm & #Hr & #Hs &
+                            #Hltr & #Hrtr & %Hoeq)".
+        Opaque isPopFiveTuple.
+        iExists p, l, m, r, s, op, ol, om, or, os, kp, kMd, ks, ltr, rtr.
+        doneL.
+        iSplit. iPureIntro. inversion conf; by easy_config.
+        iFrame "#". iFrame.
+        done.
+      - wp_bind (naive_pop_safe d)%E.
+        iApply (wp_wand with "pop_safe").
+        iIntros (true_) "->".
+        Opaque isPersFiveTuple.
         wp_pures.
         iDestruct (split_time 3 with "τ") as "[ι τ]". by lia.
-        iModIntro.
-        iFrame.
-        iExists empty_buffer,NONEV,empty_buffer,NONEV,sf'',[],[],[],[],(prC ++ mdC ++ sfC),0,0,(kSf+kMd+kPr),[],[].
-        iFrame "#".
-        iSplitR. done.
-        iSplitR.
-          { iPureIntro.
-            inversion cfg; constructor; simpl; list_elem_of.
-            - rewrite !Nat.add_0_r //.
-            - rewrite Heqpr Heqsf. list_elem_of.
-           }
-        iSplitL. by iApply three_time_enough.
-        iSplitR. by iApply empty_is_buffer_at.
-        iSplitR. by isEmptyDeque.
-        iSplitR. by iApply empty_is_buffer_at.
-        iSplitR. by isEmptyDeque.
-        do 2 doneL.
-        iDestruct (big_sepL2_nil_inv_r with "Hltr") as "->".
-        iDestruct (big_sepL2_nil_inv_r with "Hrtr") as "->".
-        iPureIntro.
-        rewrite Heq //.
-      + apply bool_decide_eq_false_1 in Heqb as Heqsf.
-        apply bool_decide_code_false in Heqb as ->.
-        wp_pures.
-        inversion cfg. symmetry in H2; by contradiction.
-        wp_apply (bpop_spec2 with "Hmd") as "%a %m %oM (#hM' & %HmdC)".
-        wp_pures.
-        wp_apply (binject_spec2 with "Hpr") as "%p' #Hp'".
-        wp_pures.
-        change (kSf ∈ map S [2; 3; 4; 5]) in H0.
-        apply decrease_in in H0 as (kSf' & -> & HkSf').
-        wp_apply (bpop_spec2 with "Hsf") as "%b %s' %oS' (#hS' & %HsfC)".
-        wp_pures.
-        wp_apply (binject_spec2 with "hM'") as "%md' #Hmd'".
-        wp_pures.
-        iModIntro.
-        iDestruct (split_time 3 with "τ") as "[ι τ]". by lia.
-        iFrame.
-        iExists p', NONEV, md', NONEV, s',
-          (prC++⋅a), [], (oM++⋅b), [], oS', (S kPr), 2, kSf', [], [].
-        iFrame "#".
-        iSplitR. done.
-        iSplitR.
-          { iPureIntro.
-            constructor;
-            [rewrite Heqpr | invert_all_in];
-            list_elem_of;
-            exfalso; apply Heqsf; by auto.
-          }
-        iSplitL. by iApply three_time_enough.
-        iSplitR. by isEmptyDeque.
-        iSplitR. by isEmptyDeque.
-        iDestruct (big_sepL2_nil_inv_r with "Hltr") as "->".
-        iDestruct (big_sepL2_nil_inv_r with "Hrtr") as "->".
-        do 2 doneL.
-        iPureIntro.
-        aac_rewrite Heq.
-        aac_rewrite HsfC.
-        aac_rewrite HmdC.
-        rewrite /= !cons_middle. aac_reflexivity.
-        *)
-      admit.
-    - wp_apply (ssref_read π _ (isPersFiveTuple _ _ _) with "[Hrd O]") as "%right
-        [(%pr1 & %ld1 & %md1 & %rd1 & %sf1 & %prC1 & %ldC1 & %mdC1 & %rdC1 & %sfC1
-            & %kPr1 & %kMd1 & %kSf1 & %ltr1 & %rtr1 & -> & %cfg1
-            & #Hpr1 & #Hld1 & #Hmd1 & #Hrd1 & #Hsf1 & #Hltr1 & #Hrtr1 & %Heq1)
-        O]".
+        wp_bind (#ℓ <- d)%E.
+        iApply (wp_wand with "[DONE ι O Hd]").
         {
-          iSplitR. iExact "Hrd".
-          iFrame.
-          iIntros (v) "H".
-          iApply (persist_structure with "H").
+          iApply ("DONE" with "[ι Hd]"); [| by iFrame].
+          iNext.
+          iApply strutcure_and_time.
+          by iFrame.
         }
-        rewrite /inspect_first /naive_pop.
-        remember (S depth) as sDepth.
-        wp_pures.
-        wp_apply (bsize_better_spec with "Hmd1") as "_".
-        wp_pures.
-        destruct (bool_decide (kMd1 = 0)) eqn:?.
-        + apply bool_decide_eq_true_1 in Heqb as Heqmd1.
-          apply bool_decide_code_true in Heqb as ->.
-          wp_pures.
-          inversion cfg1; [| exfalso; lia].
-          change (kSf1 ∈ map S [0;1;2;3;4;5;6;7]) in H3.
-          apply decrease_in in H3 as (kSf' & -> & HkSf').
-          iCombine "Hsf1 Hsf1" as "[_ #sHsf1]".
-          rewrite {11}HeqsDepth /=.
-          wp_apply (bpop_spec2 with "Hsf1") as "%x' %str' %rstr (#Hstr' & ->)".
-          wp_pures.
-          wp_alloc _ignored as "_". wp_pures. clear _ignored.
-          assert (x' ∈ rtr) as Hx'.
-            { rewrite Heq1.
-              do 4 (apply elem_of_list_app; right).
-              apply elem_of_list_app; left.
-              by list_elem_of. }
-          iDestruct (lookup_triple (S depth) _ _ _ Hx' with "Hrtr") as "(%xC' & Hx')".
-          rewrite triple_unfold.
-          iDestruct "Hx'" as "(%fst & %child & %last & %fstC & %childC & %lastC & %kFst & %kLst & %chTr & %bCfg & -> & #Hfst & #Hch & #Hlst & #chCchT & ->)".
-          wp_pures.
-          wp_bind (first_nonempty _)%E.
-          wp_apply (wp_strong_mono _ _ _ _ _ (λ v, ⌜ v = SOMEV fst ⌝)%I); [ done | done | | ].
-          {
-            rewrite /first_nonempty. wp_pures.
-            wp_apply (bsize_better_spec with "Hfst") as "_".
-            wp_pures.
-            assert (bool_decide (#kFst = #0%nat) = false) as ->.
-              { inversion bCfg; invert_all_in. }
-            wp_pures.
-            done.
+        iIntros (unit) "O".
+        wp_pures; clear unit.
+        wp_apply (safe_naive_pop with "[τ]") as (x' d' o') "(Hd' & %Heq)".
+          { iFrame "#".
+            split_t (kp ∘ ks); [| done].
+            destruct (buffer_colour (kp-1));
+            destruct (buffer_colour ks);
+            destruct (buffer_colour kp);
+            simpl; auto with arith.
           }
-          iIntros "%TMP ->". iModIntro.
-          wp_pures.
-          wp_apply (bsize_better_spec with "Hfst") as "_".
-          wp_pures.
-          destruct (bool_decide (kFst = 3%nat)) eqn:?.
-          * (* *) apply bool_decide_eq_true_1 in Heqb as Heqkfst.
-            apply bool_decide_code_true in Heqb as deckfst.
-            rewrite deckfst.
-            wp_pures.
-            wp_apply (bsize_better_spec with "Hmd1") as "_".
-            wp_pures.
-            iDestruct "sHsf1" as "[#rHsf1 %lHsf1]".
-            wp_apply (bpop_spec with "rHsf1") as "%str'' #Hstr''".
-            wp_pures.
-            wp_alloc ℓr as "Hℓr".
-            wp_pures.
-            wp_apply (bsize_better_spec with "Hfst") as "_". wp_pures.
-            wp_apply (bsize_better_spec with "Hlst") as "_". wp_pures.
-            rewrite deckfst.
-            wp_pures.
-            inversion cfg. { exfalso. apply Heqmd. done. }
-            wp_apply (bpop_spec2 with "Hmd") as "%a %m %oM (Hm & %HmdC)".
-            wp_pures.
-            wp_apply (binject_spec2 with "Hpr") as "%p' #Hp'".
-            wp_pures.
-            rewrite Heqkfst.
-            wp_apply (bpop_spec2 with "Hfst") as "%b %x' %oX' (#Hx' & %HfstC)".
-            wp_pures.
-            wp_apply (binject_spec2 with "Hm") as "%m' #Hm'".
-            wp_pures.
-            wp_bind (push _)%E.
-            rewrite /push.
-            wp_pures.
-            iDestruct (split_time 1 with "τ") as "[ι τ]". by lia.
-            wp_apply (tick_spec with "ι") as "_".
-            wp_pures.
-            wp_load.
-            wp_pures.
-            wp_apply (bsize_better_spec with "Hmd1") as "_".
-            wp_pures.
-            wp_apply (bsize_spec with "Hstr''") as "_".
-            simpl in lHsf1. inversion lHsf1.
-            rewrite H12.
-            wp_pures.
-            assert (bool_decide (#kSf' = #8%nat) = false) as ->.
-              { apply bool_decide_code_false, bool_decide_eq_false_2.
-                intro; clear H3 H5.
-                invert_all_in; lia.
-              }
-            wp_pures.
-            wp_store.
-            wp_bind (bpush _ _).
-            wp_apply (bpush_spec with "Hstr''") as "%str''' #Hstr'''".
-            wp_pures.
-            iDestruct (split_time 3 with "τ") as "[ι τ]". by lia.
-            wp_bind (ref _)%E.
-            wp_apply (ssref_alloc π (fiveTuple π (S depth) _) with "[ι]") as "%ℓ'' #Hℓ''".
-            { iExists pr1, ld1, md1, rd1, str''', oPr1, oLd1, oMd1, oRd1, _,
-                kPr1, kMd1, (S kSf').
-              rewrite -H -H0 -H1 -H2 -HeqsDepth.
-              iFrame "#". iFrame.
-              rewrite HeqsDepth.
-              iSplitR. done.
-              iSplitR.
-              {
-                iPureIntro.
-                constructor.
-                invert_all_in; list_elem_of.
-              }
-              iSplitL. by iApply three_time_enough.
-              iSplitL.
-              - iExists ((x',child,last)%V::str), ((oX'++childC++lastC)::strC).
-                iSplitL. iExact "Hstr'''".
-                iSplitL. iPureIntro. split.
-                + done.
-                + rewrite -Hlstr. by simpl.
-                + iApply big_sepL2_cons.
-                  iSplitL.
-                  * rewrite -HeqsDepth. iNext.
-                    rewrite triple_unfold.
-                    iExists x', child, last, oX', childC, lastC, 2, kLst.
-                    iSplitR.
-                      { iPureIntro.
-                        clear HkSf' H3 H5.
-                        inversion bCfg; constructor; invert_all_in;
-                        list_elem_of.
-                      }
-                    iSplitR. done.
-                    rewrite HeqsDepth.
-                    iFrame "#".
-                    iPureIntro. done.
-                  * iApply (big_sepL2_mono with "Hstrrest").
-                    intros. iIntros "H". by iNext.
-              - iPureIntro. done.
-            }
-            wp_pures.
-            iFrame.
-            iExists p', NONEV, m', (SOMEV #ℓ''), sf,
-              (prC ++ oA), [], (oM ++ oB), _, sfC,
-              (S kPr), 2, kSf.
-            iModIntro.
-            iFrame "#"; iFrame.
-            iSplitR. done.
-            iSplitR.
-              { iPureIntro.
-                clear HkSf'.
-                constructor; invert_all_in; list_elem_of;
-                exfalso; lia.
-              }
-            iSplitL. iApply three_time_enough.
-              iDestruct (split_time 3 with "τ") as "[A _]"; by [lia | done].
-            iSplitR. by isEmptyDeque.
-            iSplitR. ℓisDeque ℓ''. by iExact "Hℓ''".
-            iDestruct (empty_buffer_is_empty with "Hpr1") as "->".
-            iDestruct (empty_buffer_is_empty with "Hmd1") as "->".
-            destruct oLd1; [| inversion H].
-            destruct oRd1; [| inversion H1].
-            iPureIntro.
-            rewrite Heq HmdC Ho1 Hos1 HoB HfstC /=.
-            aac_reflexivity.
-            *)
-            admit.
-          * apply bool_decide_eq_false_1 in Heqb as Heqkfst.
-            apply bool_decide_code_false in Heqb as deckfst.
-            rewrite deckfst.
-            wp_pures.
-            iDestruct (isDeque_unfold with "Hch") as "[[-> ->] | (%ℓi & -> & Hch')]"; wp_pures.
-            --
+        inversion Heq.
+        iApply "Hψ".
+        by iFrame.
+      Transparent isPersFiveTuple.
+    }
+    iDestruct "Unsafe" as "[Hunsafe pop_unsafe]".
+    wp_bind (naive_pop_safe d)%E.
+    iApply (wp_wand with "pop_unsafe").
+    iIntros (false_) "->".
+    wp_pures.
+    wp_apply (prepare_pop_spec with "[τ O Hunsafe]").
+    - iFrame.
+      iIntros (ℓ' x' o') "Hℓ' τ O".
+      Transparent pop_nonempty.
+      rewrite /pop_nonempty.
+      iApply ("iH" with "[Hℓ'] [τ] [O]"); iClear "iH"; try done.
+      + rewrite -isDeque_unfold. ℓisDeque ℓ'. iExact "Hℓ'".
+      + iNext.
+        iIntros (d') "[Hd O]".
+        iExists d'. iFrame. done.
+    - iIntros (f' kp ks) "(Hf' & O & τ)". iClear "iH".
+      wp_pures.
+      wp_bind (#ℓ <- f')%E.
+      Transparent isPopFiveTuple.
+      iDestruct "Hf'" as "(%p & %l & %m & %r & %s & %op & %ol & %om & %or & %os &
+                          %kMd & %ltr & %rtr &
+                          -> & %conf & #Hp & #Hl & #Hm & #Hr & #Hs &
+                          #Hltr & #Hrtr & %Hoeq)".
+      split_t (kp ⋄ ks).
+      iApply (wp_wand with "[DONE O ι]").
+      {
+        iApply ("DONE" with "[ι]"); [| done].
+        iNext.
+        iExists p, l, m, r, s, op, ol, om, or, os, kp, kMd, ks, ltr, rtr.
+        doneL.
+        iSplit. iPureIntro. inversion conf; by easy_config.
+        iFrame "#". iFrame.
+        iSplit. iApply (big_sepL2_mono with "Hltr"). by auto.
+        iSplit. iApply (big_sepL2_mono with "Hrtr"). by auto.
+        done.
+      }
+      iIntros (unit) "O". wp_pures; clear unit.
+      wp_apply (safe_naive_pop with "[τ]").
+      + split_t (kp ∘ ks).
+        iFrame.
+        iExists p, l, m, r, s, op, ol, om, or, os, kMd, ltr, rtr.
+        doneL.
+        iSplit. iPureIntro. inversion conf; by easy_config.
+        iFrame "#". iFrame.
+        iSplit. iApply (big_sepL2_mono with "Hltr"). by auto.
+        iSplit. iApply (big_sepL2_mono with "Hrtr"). by auto.
+        done.
+      + iIntros (x' d' o') "[Hd %Heq]".
+        inversion Heq.
+        iApply "Hψ".
+        iFrame.
+  Qed.
 
-End proof.
-From iris.heap_lang Require Import lang proofmode notation.
-From iris.bi Require Import derived_laws.
-
-From Coq Require Import List.
-Import ListNotations.
-
-From AAC_tactics Require Import AAC.
-From AAC_tactics Require Import Instances.
-Import Instances.Lists.
-
-From Deque Require Import common tick shared_ref deque_cost push_cost concat_cost.
-
-Section proof.
-
-  Context `{!heapGS Σ} `{!na_invG Σ}.
-  Context {π : gname}.
-
-  (* TODO: start here*)
-  Lemma pop_spec_helper oD x ℓ : forall depth,
-    {{{ isDeque π depth (⋅x ++ oD) (SOMEV #ℓ) ∗ ⏱ time_for_pop ∗ Token π depth }}}
-      pop (SOMEV #ℓ)
-    {{{ d', RET (x, d')%V; isDeque π depth oD d' ∗ Token π depth }}}.
+  Definition pop_spec : forall x o d,
+    {{{ IsDeque π (⋅x ++ o) d ∗ Token π 0 ∗ ⏱ time_for_pop }}}
+      pop d
+    {{{ d', RET (x, d')%V; IsDeque π o d' ∗ Token π 0 }}}.
   Proof.
-    iIntros (depth ψ) "(Hd & τ & O) Hψ".
-    rewrite isDeque_unfold.
+    iIntros (x o d ψ) "(#Hd & O & τ) hψ".
     rewrite /pop.
-    iLöb as "iH" forall (ℓ oD x depth).
-    iDestruct "Hd" as "[[%H _] | (%ℓ' & -> & Hℓ)]". by inversion H.
     wp_pures.
-    iDestruct (split_time 1 with "τ") as "[ι τ]". by lia.
-    wp_apply (tick_spec with "ι") as "_".
+    rewrite /IsDeque isDeque_unfold.
+    iCombine "Hd Hd" as "[_ [[-> %Heq]|(%ℓ & -> & Hℓ)]]";
+      rewrite -isDeque_unfold;
+      [ inversion Heq |].
     wp_pures.
-    wp_apply (ssref_load_open with "[Hℓ O]") as "%d (O & πd & DONE)". by iFrame.
-    iDestruct (persist_structure with "πd") as "[#Hv
-        (%pr & %ld & %md & %rd & %sf & %prC & %ldC & %mdC & %rdC & %sfC
-            & %kPr & %kMd & %kSf & %ltr & %rtr & -> & %cfg & pot
-            & #Hpr & #Hld & #Hmd & #Hrd & #Hsf & #Hltr & #Hrtr & %Heq)]".
-    wp_pures.
-    wp_bind (if: _ then _ else _)%E.
-    wp_apply (wp_strong_mono _ _ _ _ _
-      (λ v, isPopFiveTuple π depth (⋅x ++ oD) v ∗ Token π (S depth))%I
-      with "[O τ]"); [easy | easy | |]. {
-    wp_apply (bsize_better_spec with "Hmd") as "_".
-    wp_pures.
-    destruct (bool_decide (kMd = 0)) eqn:?.
-    { (* apply bool_decide_eq_true_1 in Heqb as Heqmd.
-      apply bool_decide_code_true in Heqb as ->.
-      wp_pures.
-      iDestruct (split_time 3 with "τ") as "[ι τ]". by lia.
-      iFrame.
-      inversion cfg; [| exfalso; lia].
-      destruct ldC; inversion H.
-      destruct rdC; inversion H1.
-      iDestruct (big_sepL2_nil_inv_l with "Hltr") as "->".
-      iDestruct (big_sepL2_nil_inv_l with "Hrtr") as "->".
-      iExists pr,ld,md,rd,sf,prC,[],mdC,[],sfC,0,0,kSf,[],[].
-      iFrame "#".
-      iSplitR. done.
-      iSplitR.
-        { iPureIntro.
-          rewrite Heqmd in cfg |- *.
-          invert_all_in; constructor; list_elem_of.
-        }
-      iSplitL. by iApply three_time_enough.
-      do 2 doneL.
-      done.
-      *)
-      admit.
-    }
-    apply bool_decide_eq_false_1 in Heqb as Heqmd.
-    apply bool_decide_code_false in Heqb as ->.
-    wp_pures.
-    wp_apply (bsize_better_spec with "Hpr") as "_".
-    wp_pures.
-    destruct (bool_decide (kPr = 3)) eqn:?.
-    2: { (*
-      apply bool_decide_eq_false_1 in Heqb as Heqpr.
-      apply bool_decide_code_false in Heqb as ->.
-      wp_pures.
-      iDestruct (split_time 3 with "τ") as "[ι τ]". by lia.
-      iFrame.
-      iExists pr,ld,md,rd,sf,prC,ldC,mdC,rdC,sfC,kPr,kMd,kSf,ltr,rtr.
-      iFrame "#".
-      iSplitR. done.
-      iSplitR.
-        { iPureIntro.
-          inversion cfg; [exfalso; lia |].
-          invert_all_in; constructor; list_elem_of.
-        }
-      iSplitL. by iApply three_time_enough.
-      iSplitR. iApply (big_sepL2_mono with "Hltr"). by auto.
-      iSplitR. iApply (big_sepL2_mono with "Hrtr"). by auto.
-      done.
-      *)
-      admit.
-    }
-    apply bool_decide_eq_true_1 in Heqb as Heqpr.
-    apply bool_decide_code_true in Heqb as ->.
-    wp_pures.
-    rewrite {1}isDeque_unfold {1}isDeque_unfold.
-    iDestruct "Hld" as "[[-> ->] | (%ℓld & -> & Hld)]";
-    iDestruct "Hrd" as "[[-> ->] | (%ℓrd & -> & Hrd)]";
-    wp_pures.
-    - (* wp_apply (bsize_better_spec with "Hsf") as "_".
-      wp_pures.
-      destruct (bool_decide (kSf = 3)) eqn:?.
-      + apply bool_decide_eq_true_1 in Heqb as Heqsf.
-        apply bool_decide_code_true in Heqb as ->.
-        wp_pures.
-        wp_bind (inject_whole_buffer _ _ _).
-        wp_apply (binject_whole_spec with "[Hmd Hsf]") as "%sf' #Hsf'".
-          by iFrame "#".
-        wp_apply (binject_whole_spec with "[Hmd Hsf']") as "%sf'' #Hsf''".
-          by iFrame "#".
-        wp_pures.
-        iDestruct (split_time 3 with "τ") as "[ι τ]". by lia.
-        iModIntro.
-        iFrame.
-        iExists empty_buffer,NONEV,empty_buffer,NONEV,sf'',[],[],[],[],(prC ++ mdC ++ sfC),0,0,(kSf+kMd+kPr),[],[].
-        iFrame "#".
-        iSplitR. done.
-        iSplitR.
-          { iPureIntro.
-            inversion cfg; constructor; simpl; list_elem_of.
-            - rewrite !Nat.add_0_r //.
-            - rewrite Heqpr Heqsf. list_elem_of.
-           }
-        iSplitL. by iApply three_time_enough.
-        iSplitR. by iApply empty_is_buffer_at.
-        iSplitR. by isEmptyDeque.
-        iSplitR. by iApply empty_is_buffer_at.
-        iSplitR. by isEmptyDeque.
-        do 2 doneL.
-        iDestruct (big_sepL2_nil_inv_r with "Hltr") as "->".
-        iDestruct (big_sepL2_nil_inv_r with "Hrtr") as "->".
-        iPureIntro.
-        rewrite Heq //.
-      + apply bool_decide_eq_false_1 in Heqb as Heqsf.
-        apply bool_decide_code_false in Heqb as ->.
-        wp_pures.
-        inversion cfg. symmetry in H2; by contradiction.
-        wp_apply (bpop_spec2 with "Hmd") as "%a %m %oM (#hM' & %HmdC)".
-        wp_pures.
-        wp_apply (binject_spec2 with "Hpr") as "%p' #Hp'".
-        wp_pures.
-        change (kSf ∈ map S [2; 3; 4; 5]) in H0.
-        apply decrease_in in H0 as (kSf' & -> & HkSf').
-        wp_apply (bpop_spec2 with "Hsf") as "%b %s' %oS' (#hS' & %HsfC)".
-        wp_pures.
-        wp_apply (binject_spec2 with "hM'") as "%md' #Hmd'".
-        wp_pures.
-        iModIntro.
-        iDestruct (split_time 3 with "τ") as "[ι τ]". by lia.
-        iFrame.
-        iExists p', NONEV, md', NONEV, s',
-          (prC++⋅a), [], (oM++⋅b), [], oS', (S kPr), 2, kSf', [], [].
-        iFrame "#".
-        iSplitR. done.
-        iSplitR.
-          { iPureIntro.
-            constructor;
-            [rewrite Heqpr | invert_all_in];
-            list_elem_of;
-            exfalso; apply Heqsf; by auto.
-          }
-        iSplitL. by iApply three_time_enough.
-        iSplitR. by isEmptyDeque.
-        iSplitR. by isEmptyDeque.
-        iDestruct (big_sepL2_nil_inv_r with "Hltr") as "->".
-        iDestruct (big_sepL2_nil_inv_r with "Hrtr") as "->".
-        do 2 doneL.
-        iPureIntro.
-        aac_rewrite Heq.
-        aac_rewrite HsfC.
-        aac_rewrite HmdC.
-        rewrite /= !cons_middle. aac_reflexivity.
-        *)
-      admit.
-    - wp_apply (ssref_read π _ (isPersFiveTuple _ _ _) with "[Hrd O]") as "%right
-        [(%pr1 & %ld1 & %md1 & %rd1 & %sf1 & %prC1 & %ldC1 & %mdC1 & %rdC1 & %sfC1
-            & %kPr1 & %kMd1 & %kSf1 & %ltr1 & %rtr1 & -> & %cfg1
-            & #Hpr1 & #Hld1 & #Hmd1 & #Hrd1 & #Hsf1 & #Hltr1 & #Hrtr1 & %Heq1)
-        O]".
-        {
-          iSplitR. iExact "Hrd".
-          iFrame.
-          iIntros (v) "H".
-          iApply (persist_structure with "H").
-        }
-        rewrite /inspect_first /naive_pop.
-        remember (S depth) as sDepth.
-        wp_pures.
-        wp_apply (bsize_better_spec with "Hmd1") as "_".
-        wp_pures.
-        destruct (bool_decide (kMd1 = 0)) eqn:?.
-        + apply bool_decide_eq_true_1 in Heqb as Heqmd1.
-          apply bool_decide_code_true in Heqb as ->.
-          wp_pures.
-          inversion cfg1; [| exfalso; lia].
-          change (kSf1 ∈ map S [0;1;2;3;4;5;6;7]) in H3.
-          apply decrease_in in H3 as (kSf' & -> & HkSf').
-          iCombine "Hsf1 Hsf1" as "[_ #sHsf1]".
-          rewrite {11}HeqsDepth /=.
-          wp_apply (bpop_spec2 with "Hsf1") as "%x' %str' %rstr (#Hstr' & ->)".
-          wp_pures.
-          wp_alloc _ignored as "_". wp_pures. clear _ignored.
-          assert (x' ∈ rtr) as Hx'.
-            { rewrite Heq1.
-              do 4 (apply elem_of_list_app; right).
-              apply elem_of_list_app; left.
-              by list_elem_of. }
-          iDestruct (lookup_triple (S depth) _ _ _ Hx' with "Hrtr") as "(%xC' & Hx')".
-          rewrite triple_unfold.
-          iDestruct "Hx'" as "(%fst & %child & %last & %fstC & %childC & %lastC & %kFst & %kLst & %chTr & %bCfg & -> & #Hfst & #Hch & #Hlst & #chCchT & ->)".
-          wp_pures.
-          wp_bind (first_nonempty _)%E.
-          wp_apply (wp_strong_mono _ _ _ _ _ (λ v, ⌜ v = SOMEV fst ⌝)%I); [ done | done | | ].
-          {
-            rewrite /first_nonempty. wp_pures.
-            wp_apply (bsize_better_spec with "Hfst") as "_".
-            wp_pures.
-            assert (bool_decide (#kFst = #0%nat) = false) as ->.
-              { inversion bCfg; invert_all_in. }
-            wp_pures.
-            done.
-          }
-          iIntros "%TMP ->". iModIntro.
-          wp_pures.
-          wp_apply (bsize_better_spec with "Hfst") as "_".
-          wp_pures.
-          destruct (bool_decide (kFst = 3%nat)) eqn:?.
-          * (* *) apply bool_decide_eq_true_1 in Heqb as Heqkfst.
-            apply bool_decide_code_true in Heqb as deckfst.
-            rewrite deckfst.
-            wp_pures.
-            wp_apply (bsize_better_spec with "Hmd1") as "_".
-            wp_pures.
-            iDestruct "sHsf1" as "[#rHsf1 %lHsf1]".
-            wp_apply (bpop_spec with "rHsf1") as "%str'' #Hstr''".
-            wp_pures.
-            wp_alloc ℓr as "Hℓr".
-            wp_pures.
-            wp_apply (bsize_better_spec with "Hfst") as "_". wp_pures.
-            wp_apply (bsize_better_spec with "Hlst") as "_". wp_pures.
-            rewrite deckfst.
-            wp_pures.
-            inversion cfg. { exfalso. apply Heqmd. done. }
-            wp_apply (bpop_spec2 with "Hmd") as "%a %m %oM (Hm & %HmdC)".
-            wp_pures.
-            wp_apply (binject_spec2 with "Hpr") as "%p' #Hp'".
-            wp_pures.
-            rewrite Heqkfst.
-            wp_apply (bpop_spec2 with "Hfst") as "%b %x' %oX' (#Hx' & %HfstC)".
-            wp_pures.
-            wp_apply (binject_spec2 with "Hm") as "%m' #Hm'".
-            wp_pures.
-            wp_bind (push _)%E.
-            rewrite /push.
-            wp_pures.
-            iDestruct (split_time 1 with "τ") as "[ι τ]". by lia.
-            wp_apply (tick_spec with "ι") as "_".
-            wp_pures.
-            wp_load.
-            wp_pures.
-            wp_apply (bsize_better_spec with "Hmd1") as "_".
-            wp_pures.
-            wp_apply (bsize_spec with "Hstr''") as "_".
-            simpl in lHsf1. inversion lHsf1.
-            rewrite H12.
-            wp_pures.
-            assert (bool_decide (#kSf' = #8%nat) = false) as ->.
-              { apply bool_decide_code_false, bool_decide_eq_false_2.
-                intro; clear H3 H5.
-                invert_all_in; lia.
-              }
-            wp_pures.
-            wp_store.
-            wp_bind (bpush _ _).
-            wp_apply (bpush_spec with "Hstr''") as "%str''' #Hstr'''".
-            wp_pures.
-            iDestruct (split_time 3 with "τ") as "[ι τ]". by lia.
-            wp_bind (ref _)%E.
-            wp_apply (ssref_alloc π (fiveTuple π (S depth) _) with "[ι]") as "%ℓ'' #Hℓ''".
-            { iExists pr1, ld1, md1, rd1, str''', oPr1, oLd1, oMd1, oRd1, _,
-                kPr1, kMd1, (S kSf').
-              rewrite -H -H0 -H1 -H2 -HeqsDepth.
-              iFrame "#". iFrame.
-              rewrite HeqsDepth.
-              iSplitR. done.
-              iSplitR.
-              {
-                iPureIntro.
-                constructor.
-                invert_all_in; list_elem_of.
-              }
-              iSplitL. by iApply three_time_enough.
-              iSplitL.
-              - iExists ((x',child,last)%V::str), ((oX'++childC++lastC)::strC).
-                iSplitL. iExact "Hstr'''".
-                iSplitL. iPureIntro. split.
-                + done.
-                + rewrite -Hlstr. by simpl.
-                + iApply big_sepL2_cons.
-                  iSplitL.
-                  * rewrite -HeqsDepth. iNext.
-                    rewrite triple_unfold.
-                    iExists x', child, last, oX', childC, lastC, 2, kLst.
-                    iSplitR.
-                      { iPureIntro.
-                        clear HkSf' H3 H5.
-                        inversion bCfg; constructor; invert_all_in;
-                        list_elem_of.
-                      }
-                    iSplitR. done.
-                    rewrite HeqsDepth.
-                    iFrame "#".
-                    iPureIntro. done.
-                  * iApply (big_sepL2_mono with "Hstrrest").
-                    intros. iIntros "H". by iNext.
-              - iPureIntro. done.
-            }
-            wp_pures.
-            iFrame.
-            iExists p', NONEV, m', (SOMEV #ℓ''), sf,
-              (prC ++ oA), [], (oM ++ oB), _, sfC,
-              (S kPr), 2, kSf.
-            iModIntro.
-            iFrame "#"; iFrame.
-            iSplitR. done.
-            iSplitR.
-              { iPureIntro.
-                clear HkSf'.
-                constructor; invert_all_in; list_elem_of;
-                exfalso; lia.
-              }
-            iSplitL. iApply three_time_enough.
-              iDestruct (split_time 3 with "τ") as "[A _]"; by [lia | done].
-            iSplitR. by isEmptyDeque.
-            iSplitR. ℓisDeque ℓ''. by iExact "Hℓ''".
-            iDestruct (empty_buffer_is_empty with "Hpr1") as "->".
-            iDestruct (empty_buffer_is_empty with "Hmd1") as "->".
-            destruct oLd1; [| inversion H].
-            destruct oRd1; [| inversion H1].
-            iPureIntro.
-            rewrite Heq HmdC Ho1 Hos1 HoB HfstC /=.
-            aac_reflexivity.
-            *)
-            admit.
-          * apply bool_decide_eq_false_1 in Heqb as Heqkfst.
-            apply bool_decide_code_false in Heqb as deckfst.
-            rewrite deckfst.
-            wp_pures.
-            iDestruct (isDeque_unfold with "Hch") as "[[-> ->] | (%ℓi & -> & Hch')]"; wp_pures.
-            --
+    wp_apply (pop_spec_helper with "[O τ]").
+      by (iFrame; iFrame "#").
+    done.
+  Qed.
 
 End proof.
